# 01 Different Derivations (Lab)

Consider again grammar `Gâ‚€`. Give two _different_ derivations of `Dave runs`.

First derivation:

S â†’ NP VP
â†’PN VP
â†’Dave V
â†’Dave runs

Second derivation:
S â†’NP VP
â†’PN VP
â†’PN V
â†’PN runs
â†’Dave runs

# 02 Equivalent Languages (Lab)

Let `Gâ‚‚' = (T, N, P, S)` with `T = {a}`, `N = {S}` productions `P`:

```
S â†’ Îµ
S â†’ Sa
```

Prove that `L(Gâ‚‚') = {aâ¿ | n â‰¥ 0}`, which is the same as `L(Gâ‚‚)` from the course notes.

We prove this formally by inclusion in both directions. By definition of `L(Gâ‚‚)`,

```
{Ï‡ âˆˆ T* | S â‡’á© Ï‡} âŠ† {aâ¿ | n â‰¥ 0}
```

means that for every `Ï‡ âˆˆ T*` that is derivable from `S` there exists an `n â‰¥ 0` such that `Ï‡ = aâ¿`. We show this by induction over the length of derivations.

-   _Base._ Suppose `Ï‡` is derived directly from `S` by `S â‡’ Ï‡`, which leaves only `Ï‡ = Îµ` according to the first production. Then `Ï‡ = aâ°`.
-   _Step._ Suppose `Ï‡` is derived from `S` in multiple steps, which leaves only `S â‡’ Sa â‡’* Ï‡` according to the second production. Then `Ï‡` must be `Ï‰a` to be derivable from `Sa`. As the derivation `S â‡’* Ï‰` is shorter than the derivation of `S â‡’* Ï‡`, by induction assumption there exists an `n` such that `Ï‰ = aâ¿`. Therefore `Ï‡ = Ï‰a = aâ¿a = aâ¿âºÂ¹`.

The inclusion in the other direction means that every `aâ¿` for `n â‰¥ 0` can be derived from `S`:

```
{aâ¿ | n â‰¥ 0} âŠ† {Ï‡ âˆˆ T* | S â‡’á© Ï‡}
```

We show this by induction over `n`.

-   _Base._ obviously `aâ° = Îµ` can be generated by the first production, `S â‡’á© Îµ`.
-   _Step._ Suppose `aâ¿` can be generated, `S â‡’á© aâ¿`. We need to show that `aâ¿âºÂ¹` can be generated as well. This follows from `S â‡’ Sa â‡’á© aâ¿a = aâ¿âºÂ¹`.

Thus, we can conclude `L(Gâ‚‚)' = {aâ¿ | n â‰¥ 0}`.

# 03 Derivation in Copy Language (Lab)

S

$\rightarrow$ aAS

$\rightarrow$ aAbBS

$\rightarrow$ abASb

$\rightarrow$ abAbBSb

$\rightarrow$ abbABSb

$\rightarrow$ abbASbb

$\rightarrow$ abbSabb

$\rightarrow$ abbabb

# 04 Ambiguity in English (Lab)

A well-known syntactically ambiguous English sentence is `Time flies like an arrow`. Explain the ambiguity!

[ Time flies ] like [an arrow], i.e the species of time flies happen to like an arrow or

TIme [flies [like [an arrow]]], i.e time flies figurateively very fast like an arrorw.

First interpretation does not semantically make sense.


# 05 Extending English Grammar (Lab)

Define a new grammar `Gâ‚€'` by extending `Gâ‚€`:

-   A verb phrase is a verb phrase followed by a prepositional phrase.
-   A prepositional phrase is a preposition followed by a noun phrase.
-   Prepositions are `in` and `on`.
-   Nouns are `park` and `child`.

Give the full definition of `Gâ‚€'`! Is `Gâ‚€'` regular, context-free, or context-sensitive? Draw the parse tree of `the child eats a banana in the park`! Use [draw.io](https://draw.io) or a similar program to generate an SVG figure and insert that in the cell below. 

ğºâ€²0=(ğ‘‡,ğ‘,ğ‘ƒ,ğ‘†)

ğ‘‡

= (Kevin, Dave, a, the, banana, apple, eats, runs, park, child, in, on)

ğ‘=ğ‘†,ğ‘ğ‘ƒ,ğ‘‰ğ‘ƒ,ğ‘ƒğ‘ƒ,ğ‘ƒğ‘,ğ·,ğ‘,ğ‘‰,ğ‘ƒ

Grammar Definition:

S â†’NP VP
NP â†’PN
NP â†’D N
VP â†’V
VP â†’VP NP
VP â†’VP PP
PP â†’P NP
PN â†’Kevin
PN â†’Dave
D â†’a
D â†’the
P â†’in
P â†’on
N â†’banana
N â†’apple
N â†’park
N â†’child
V â†’eats
V â†’runs

ğºâ€²0 is not regular, but it is context-free.

Derivation:
S â†’NP VP
â†’D N VP PP
â†’the child VP NP P NP
â†’the child VP D N P NP
â†’the child V D N P NP
â†’the child eats a banana P NP
â†’the child eats a banana in D N
â†’the child eats a banana in the park

![[q5.drawio.svg]]


# 06 Generated Language aâ¿bcâ¿ (Lab)

Prove formally that `L(Gâ‚ƒ) = {aâ¿bcâ¿ | n â‰¥ 0}`! [8 points]

We prove this formally by inclusion in both directions. By definition of $L\left(G_3\right)$.

$$
\left\{\chi \in T^* \mid S \Rightarrow^{+} \chi\right\} \subseteq\left\{a^nbc^n \mid n \geq \theta\right\}
$$

means that for every $\chi \in T^*$ that is derivable from $S$ there exists an $n \geq 0$ such that $\chi=a^nbc^n$. We show this by induction over the length of derivations.

- Base. Suppose $\chi$ is derived directly from $S$ by $S \Rightarrow \chi$, which leaves only $b\varepsilon = b$ according to the first production. Then $\chi=a^nbc^n{\circ}$.
- Step. Suppose $\chi$ is derived from $S$ in multiple steps, which leaves only $S \Rightarrow S abc \Rightarrow^* \chi$ according to the second production. Then $\chi$ must be $wabc$ to be derivable from $Sabc$. As the derivation $S \Rightarrow^* w$ is shorter than the derivation of $S \Rightarrow^* \chi$, by induction assumption there exists an $n$ such that $w=a^nbc^n$. Therefore $\chi=w a=a^nbc^n =a^{n+1}bc^{n+1}$.

The inclusion in the other direction means that every $a^nbc^n$ for $n \geq 0$ can be derived from $S$ :
$$
\left\{a^nbc^n \mid n \geq \theta\right\} \subseteq\left\{\chi \in T^* \mid S \Rightarrow^{+} \chi\right\}
$$

We show this by induction over $n$.

- Base, obviously $a^{\circ}bc^{\circ}=\varepsilon$ can be generated by the first production, ${a^{+}bc^{+}} \varepsilon$.
- Step. Suppose $a^nbc^n$ can be generated, $S \Rightarrow^{+} a^nbc^n$. We need to show that $a^{n+1}bc^{n+1}$ can be generated as well. This follows from $S \Rightarrow S a \Rightarrow^{+} a^nbc^n a=a^{n+1}bc^{n+1}$.

Thus we can conclude $L\left(G_3\right)^{\prime}=\left\{a^nbc^n \mid n \geq \theta\right\}$.

